theories/coneris/examples/hash/con_hash_interface0.v
@@ -19,30 +19,42 @@ Class con_hash0 `{!conerisGS Σ} (val_size:nat):= Con_Hash0
   (* tape_name: Type; *)
   
   hash_view_gname:Type;
-  hash_map_gname:Type;
   hash_lock_gname:Type;
   
   (** * Predicates *)
-  con_hash_inv0  (f l hm: val) (γ1:hash_view_gname) (γ2:hash_map_gname) (γ_lock:hash_lock_gname): iProp Σ;
+  con_hash_inv0 (N:namespace) (f l hm: val) (γ1:hash_view_gname)(γ_lock:hash_lock_gname): iProp Σ;
   (* concrete_seq_hash {L:seq_hashG Σ} (f:val) (m:gmap nat nat) : iProp Σ;  *)
   hash_tape0 (α:val) (ns:list nat) : iProp Σ;
-  con_hash_view0 (v res:nat) (γ:hash_view_gname): iProp Σ;
+  hash_auth0 (m:gmap nat nat) (γ2:hash_view_gname) : iProp Σ;
+  hash_frag0 (v res:nat) (γ:hash_view_gname): iProp Σ;
   
   (** * General properties of the predicates *)
   (* #[global] concrete_seq_hash_timeless {L : seq_hashG Σ} f m :: *)
   (*   Timeless (concrete_seq_hash (L:=L) f m); *)
   #[global] hash_tape_timeless α ns ::
     Timeless (hash_tape0 α ns); 
-  #[global] con_hash_view_timeless v res γ ::
-    Timeless (con_hash_view0 v res γ);
-  #[global] con_hash_inv_persistent f l hm γ1 γ2 γ_lock ::
-    Persistent (con_hash_inv0 f l hm γ1 γ2 γ_lock);
-  #[global] con_hash_view_persistent v res γ ::
-    Persistent (con_hash_view0 v res γ);
-  con_hash_view_frag_frag_agree k v1 v2 γ :
-    con_hash_view0 k v1 γ -∗ con_hash_view0 k v2 γ -∗ ⌜v1=v2⌝; 
+  #[global] hash_map_timeless m γ ::
+    Timeless (hash_auth0 m γ);
+  #[global] hash_frag_timeless v res γ ::
+    Timeless (hash_frag0 v res γ);
+  #[global] con_hash_inv_persistent N f l hm γ1 γ_lock ::
+    Persistent (con_hash_inv0 N f l hm γ1 γ_lock);
+  #[global] hash_frag_persistent v res γ ::
+    Persistent (hash_frag0 v res γ);
+  
   hash_tape_valid α ns:
     hash_tape0 α ns -∗ ⌜Forall (λ x, x<=val_size)%nat ns⌝;
+  hash_auth_exclusive m m' γ:
+    hash_auth0 m γ -∗ hash_auth0 m' γ -∗ False;
+  hash_auth_frag_agree m k v γ:
+    hash_auth0 m γ -∗ hash_frag0 k v γ -∗ ⌜m!!k = Some v⌝;
+  hash_frag_frag_agree k v1 v2 γ :
+    hash_frag0 k v1 γ -∗ hash_frag0 k v2 γ -∗ ⌜v1=v2⌝;
+  hash_auth_duplicate_frag m k v γ:
+    m!!k=Some v -> hash_auth0 m γ -∗ hash_frag0 k v γ;
+  hash_auth_insert m k v γ:
+    m!!k=None -> hash_auth0 m γ ==∗ (hash_auth0 (<[k:=v]> m) γ ∗ hash_frag0 k v γ);
+                      
 
   con_hash_presample0 E (ε:nonnegreal) ns α (ε2 : fin (S val_size) → R) :
     (∀ x : fin (S val_size), (0 <= ε2 x)%R)->
@@ -54,29 +66,76 @@ Class con_hash0 `{!conerisGS Σ} (val_size:nat):= Con_Hash0
           hash_tape0 α (ns++[fin_to_nat n]) 
       );
 
-  con_hash_init0:
+  con_hash_init0 N:
     {{{ True }}}
       init_hash0 #()
-      {{{ (f:val), RET f; ∃ l hm γ1 γ2 γ_lock, con_hash_inv0 f l hm γ1 γ2 γ_lock }}};
+      {{{ (f:val), RET f; ∃ l hm γ1 γ_lock, con_hash_inv0 N f l hm γ1 γ_lock }}};
 
   con_hash_alloc_tape0:
     {{{ True }}}
       allocate_tape0 #()
       {{{ (α: val), RET α; hash_tape0 α [] }}};
   
-  con_hash_spec0 f l hm γ1 γ2 γlock α n ns (v:nat):
-    {{{ con_hash_inv0 f l hm γ1 γ2 γlock ∗ hash_tape0 α (n::ns) }}}
+  con_hash_spec0 N f l hm γ1 γlock α ns (v:nat) P Q:
+  {{{ con_hash_inv0 N f l hm γ1 γlock ∗ hash_tape0 α (ns) ∗
+      ( ∀ m, hash_auth0 m γ1 ={⊤∖↑N}=∗
+             match m!!v with
+             | Some res => hash_auth0 m γ1 ∗ P res
+             | None => ∃ n ns', ⌜n::ns'=ns⌝ ∗ hash_auth0 (<[v:=n]> m) γ1 ∗ Q
+             end                                        
+      )
+  }}}
       f #v α
-      {{{ (res:nat), RET (#res);  con_hash_view0 v res γ1 ∗
+      {{{ (res:nat), RET (#res);  (hash_tape0 α (ns) ∗ P res ∨
+                                 ∃ n ns', ⌜n::ns'=ns⌝ ∗ hash_tape0 α ns' ∗ ⌜res=n⌝ ∗ Q 
+                                )
+      }}};
+  (* con_hash_spec_hashed_before0 f l hm γ1 γ2 γlock α ns res (v:nat): *)
+  (*   {{{ con_hash_inv0 f l hm γ1 γ2 γlock ∗ hash_tape0 α ns ∗ hash_frag0 v res γ1}}} *)
+  (*     f #v α *)
+  (*     {{{ RET (#res);  hash_frag0 v res γ1 ∗ *)
+  (*                      (hash_tape0 α ns) *)
+  (*     }}} *)
+}.
+
+Section test.
+  Context `{conerisGS Σ, !con_hash0 val_size}.
+  Lemma con_hash_spec0' N f l hm γ1 γlock α n ns (v:nat):
+    {{{ con_hash_inv0 N f l hm γ1 γlock ∗ hash_tape0 α (n::ns) }}}
+      f #v α
+      {{{ (res:nat), RET (#res);  hash_frag0 v res γ1 ∗
                                 (hash_tape0 α ns ∗ ⌜res=n⌝ ∨
                                  hash_tape0 α (n::ns)
                                 )
-      }}};
-  con_hash_spec_hashed_before0 f l hm γ1 γ2 γlock α ns res (v:nat):
-    {{{ con_hash_inv0 f l hm γ1 γ2 γlock ∗ hash_tape0 α ns ∗ con_hash_view0 v res γ1}}}
-      f #v α
-      {{{ RET (#res);  con_hash_view0 v res γ1 ∗
-                       (hash_tape0 α ns)
-      }}}
-}.
+      }}}.
+  Proof.
+    iIntros (Φ) "[#Hinv Ht] HΦ".
+    iApply (con_hash_spec0 _ _ _ _ _ _ _ _ _ (λ res, hash_frag0 v res γ1) (hash_frag0 v n γ1) with "[$Hinv $Ht]").
+    - iIntros (m) "Hauth".
+      case_match.
+      + iModIntro.
+        iDestruct (hash_auth_duplicate_frag with "[$]") as "#?"; first done.
+        by iFrame.
+      + iMod (hash_auth_insert with "[$]"); first done.
+        iFrame. iModIntro. by iExists _. 
+    - iNext. iIntros (res) "[[??]|(%&%&%&?&%&?)]"; iApply "HΦ"; iFrame.
+      simplify_eq. iFrame.
+      iLeft. by iFrame.
+  Qed.
 
+  Lemma con_hash_spec_hashed_before N f l hm γ1 γlock α ns res (v:nat):
+    {{{ con_hash_inv0 N f l hm γ1 γlock ∗ hash_tape0 α ns ∗ hash_frag0 v res γ1}}}
+      f #v α
+      {{{ RET (#res);  hash_frag0 v res γ1 ∗
+                       (hash_tape0 α ns)
+      }}}.
+  Proof.
+    iIntros (Φ) "(#Hinv & Ht & #Hfrag) HΦ".
+    iApply (con_hash_spec0 _ _ _ _ _ _ _ _ _ (λ res', ⌜res=res'⌝∗ hash_frag0 v res γ1)%I (False) with "[$Hinv $Ht]").
+    - iIntros. iDestruct (hash_auth_frag_agree with "[$][//]") as "->".
+      iFrame. iModIntro. by iSplit. 
+    - iNext. iIntros (?) "[(?&->&?)|(%&%&%&?&%&%)]"; last done.
+      iApply "HΦ".
+      iFrame.
+  Qed.
+End test.
